LambdaS5/caml/parse.ml
@@ -1,19 +1,62 @@
 open Batteries
 
+open Ljs_syntax
+
 let sprintf_pos p = Printf.sprintf "row %d col %d" p.Lexing.pos_lnum p.Lexing.pos_bol
+
+let rec check_var_scope vs e =
+  match e with
+  | Fail (_, _)
+  | Dump
+  | Empty _
+  | Null _
+  | Undefined _
+  | String _
+  | Num _
+  | True _
+  | False _ -> ()
+  | Id ((p1, p2, _), i) -> if Set.mem i vs then () else failwith (Printf.sprintf "Parse error: undefined id %s at %s" i (sprintf_pos p1))
+  | Object (_, _, l, _) -> List.iter (fun (_, e) -> check_var_scope vs e) l
+  | GetAttr (_, _, e1, e2) -> check_var_scope vs e1; check_var_scope vs e2
+  | SetAttr (_, _, e1, e2, e3) -> check_var_scope vs e1; check_var_scope vs e2; check_var_scope vs e3
+  | GetObjAttr (_, _, e1) -> check_var_scope vs e1
+  | SetObjAttr (_, _, e1, e2) -> check_var_scope vs e1; check_var_scope vs e2
+  | GetField (_, e1, e2) -> check_var_scope vs e1; check_var_scope vs e2
+  | SetField (_, e1, e2, e3) -> check_var_scope vs e1; check_var_scope vs e2; check_var_scope vs e3
+  | DeleteField (_, e1, e2) -> check_var_scope vs e1; check_var_scope vs e2
+  | GetInternal (_, _, e1) -> check_var_scope vs e1
+  | SetInternal (_, _, e1, e2) -> check_var_scope vs e1; check_var_scope vs e2
+  | OwnFieldNames (_, e1) -> check_var_scope vs e1
+  | Op1 (_, _, e1) -> check_var_scope vs e1
+  | Op2 (_, _, e1, e2) -> check_var_scope vs e1; check_var_scope vs e2
+  | If (_, e1, e2, e3) -> check_var_scope vs e1; check_var_scope vs e2; check_var_scope vs e3
+  | App (_, e1, es) -> check_var_scope vs e1; List.iter (check_var_scope vs) es
+  | Seq (_, e1, e2) -> check_var_scope vs e1; check_var_scope vs e2
+  | JSeq (_, e1, e2) -> check_var_scope vs e1; check_var_scope vs e2
+  | Let (_, s, e1, e2) -> check_var_scope vs e1; check_var_scope (Set.add s vs) e2
+  | Rec (_, s, e1, e2) -> check_var_scope (Set.add s vs) e1; check_var_scope (Set.add s vs) e2
+  | Label (_, _, e1) -> check_var_scope vs e1
+  | Break (_, _, e1) -> check_var_scope vs e1
+  | TryCatch (_, e1, e2) -> check_var_scope vs e1; check_var_scope vs e2
+  | TryFinally (_, e1, e2) -> check_var_scope vs e1; check_var_scope vs e2
+  | Throw (_, e1) -> check_var_scope vs e1
+  | Lambda (_, is, e) -> check_var_scope (Set.union (Set.of_list is) vs) e
+  | Eval (_, e1, e2) -> check_var_scope vs e1; check_var_scope vs e2
+  | Hint (_, _, e1) -> check_var_scope vs e1
 
 let parse_es5 cin name =
   let lexbuf = Lexing.from_channel cin in
     try 
       (* Set the correct filename in lexbuf (for source-tracking). *)
       lexbuf.Lexing.lex_curr_p <- { lexbuf.Lexing.lex_curr_p with Lexing.pos_fname = name };
-      Ljs_parser.prog Ljs_lexer.token lexbuf
+      let v = Ljs_parser.prog Ljs_lexer.token lexbuf in
+      check_var_scope Set.empty v; v
     with
       |  Failure "lexing: empty token" ->
            failwith "lexical error"
       | Failure "utf8_of_point not implemented" ->
         failwith "Parser doesn't do some UTF8 encoding crap"
-      | _ -> failwith (Printf.sprintf "parse error; unexpected token %s at %s"
+      | Parsing.Parse_error -> failwith (Printf.sprintf "parse error; unexpected token %s at %s"
                        (Lexing.lexeme lexbuf) (sprintf_pos (Lexing.lexeme_start_p lexbuf)))
 
 let parse_es5_env cin name =
@@ -21,13 +64,14 @@ let parse_es5_env cin name =
     try
       (* Set the correct filename in lexbuf (for source-tracking). *)
       lexbuf.Lexing.lex_curr_p <- { lexbuf.Lexing.lex_curr_p with Lexing.pos_fname = name };
-      Ljs_parser.env Ljs_lexer.token lexbuf
+      let v = Ljs_parser.env Ljs_lexer.token lexbuf in
+      check_var_scope Set.empty (v Dump); v
     with
       |  Failure "lexing: empty token" ->
            failwith "lexical error"
       | Failure "utf8_of_point not implemented" ->
         failwith "Parser doesn't do some UTF8 encoding crap"
-      | _ -> failwith (Printf.sprintf "parse error; unexpected token %s at %s"
+      | Parsing.Parse_error -> failwith (Printf.sprintf "parse error; unexpected token %s at %s"
                        (Lexing.lexeme lexbuf) (sprintf_pos (Lexing.lexeme_start_p lexbuf)))
 
 
