LambdaS5/tests/es5/arguments_getter.in.js
@@ -1,3 +1,3 @@
 var x = {get x() { return arguments.length }, set y(v) { return arguments.length }};
-print(x.x)
+print(x.x);
 print(x.y = 0)
